Foundation/Logic/HilbertStyle/Basic.lean
@@ -194,6 +194,9 @@ lemma K!_intro_iff [HasAxiomAndInst 𝓢] [HasAxiomAndElim 𝓢] : 𝓢 ⊢! φ 
 
 lemma E!_intro_iff [HasAxiomAndInst 𝓢] [HasAxiomAndElim 𝓢] : 𝓢 ⊢! φ ⭤ ψ ↔ 𝓢 ⊢! φ ➝ ψ ∧ 𝓢 ⊢! ψ ➝ φ := ⟨fun h ↦ ⟨K!_left h, K!_right h⟩, fun h ↦ K!_intro h.1 h.2⟩
 
+lemma C_of_E_mp! [HasAxiomAndInst 𝓢] [HasAxiomAndElim 𝓢] (h : 𝓢 ⊢! φ ⭤ ψ) : 𝓢 ⊢! φ ➝ ψ := by exact E!_intro_iff.mp h |>.1;
+lemma C_of_E_mpr! [HasAxiomAndInst 𝓢] [HasAxiomAndElim 𝓢] (h : 𝓢 ⊢! φ ⭤ ψ) : 𝓢 ⊢! ψ ➝ φ := by exact E!_intro_iff.mp h |>.2;
+
 lemma iff_of_E!  [HasAxiomAndInst 𝓢] [HasAxiomAndElim 𝓢] (h : 𝓢 ⊢! φ ⭤ ψ) : 𝓢 ⊢! φ ↔ 𝓢 ⊢! ψ := ⟨fun hp ↦ K!_left h ⨀ hp, fun hq ↦ K!_right h ⨀ hq⟩
 
 def C_id [HasAxiomImply₁ 𝓢] [HasAxiomImply₂ 𝓢] (φ : F) : 𝓢 ⊢ φ ➝ φ := imply₂ (φ := φ) (ψ := (φ ➝ φ)) (χ := φ) ⨀ imply₁ ⨀ imply₁
@@ -357,6 +360,7 @@ lemma right_Conj₂!_intro (φ : F) (Γ : List F) (b : (ψ : F) → ψ ∈ Γ �
 
 def CConj₂Conj₂ [DecidableEq F] {Γ Δ : List F} (h : Δ ⊆ Γ) : 𝓢 ⊢ ⋀Γ ➝ ⋀Δ :=
   right_Conj₂_intro _ _ (fun _ hq ↦ left_Conj₂_intro (h hq))
+lemma CConj₂_Conj₂! [DecidableEq F] {Γ Δ : List F} (h : Δ ⊆ Γ) : 𝓢 ⊢! ⋀Γ ➝ ⋀Δ := ⟨CConj₂Conj₂ h⟩
 
 end Conjunction
 
